src/Std/Data/DHashMap/Internal/Model.lean
@@ -420,6 +420,12 @@ def unionₘ [BEq α] [Hashable α] (m₁ m₂ : Raw₀ α β) : Raw₀ α β :=
   else
     insertListₘ m₁ (toListModel m₂.1.buckets)
 
+/-- Internal implementation detail of the hash map -/
+def interSmallerFnₘ [BEq α] [Hashable α] (m sofar : Raw₀ α β) (k : α) : Raw₀ α β :=
+  match m.getEntry?ₘ k with
+  | some kv' => sofar.insertₘ kv'.1 kv'.2
+  | none => sofar
+
 section
 
 variable {β : Type v}
@@ -514,6 +520,14 @@ theorem insert_eq_insertₘ [BEq α] [Hashable α] (m : Raw₀ α β) (a : α) (
     rw [Array.set_set, updateBucket]
     simp only [Array.uset, Array.ugetElem_eq_getElem]
   · rfl
+
+theorem interSmallerFn_eq_interSmallerFnₘ [BEq α] [Hashable α] (m sofar : Raw₀ α β) (k : α) :
+    interSmallerFn m sofar k = interSmallerFnₘ m sofar k := by
+  rw [interSmallerFn, interSmallerFnₘ]
+  rw [getEntry?_eq_getEntry?ₘ]
+  congr
+  ext
+  rw [insert_eq_insertₘ]
 
 theorem alter_eq_alterₘ [BEq α] [Hashable α] [LawfulBEq α] (m : Raw₀ α β) (a : α)
     (f : Option (β a) → Option (β a)) : m.alter a f = m.alterₘ a f := by
